examples/zmathlang/zcga/4.thy
@@ -26,7 +26,7 @@ where
 definition CS4 :: 
  "(*CS4_TYPES*) => bool"
 where 
-"CS4 (*CS5_VARIABLES*) == (PRE4)
+"CS4 (*CS4_VARIABLES*) == (PRE4)
 \<and> (PO5)"
 
 definition CS6 :: 
@@ -41,11 +41,11 @@ where
 "CS1 (*CS1_VARIABLES*) == (PRE1)
 \<and> (PO2)"
 
-definition CS6 :: 
- "(*CS6_TYPES*) => bool"
+definition CS3 :: 
+ "(*CS3_TYPES*) => bool"
 where 
-"CS6 (*CS6_VARIABLES*) == (PRE6)
-\<and> (PO7)"
+"CS3 (*CS3_VARIABLES*) == (PRE3)
+\<and> (PO4)"
 
 definition CS2 :: 
  "(*CS2_TYPES*) => bool"
@@ -57,6 +57,54 @@ definition OS1 ::
  "(OS1_TYPES*) => bool"
 where 
 "OS1 (OS1_VARIABLES*) == (O1)"
+
+lemma CS5_L1:
+"(\<exists> (*CS5_VARIABLESANDTYPES*).
+(PRE5)
+\<and> (PO6)
+\<and> (SI1)
+\<and> (SI1'))"
+sorry
+
+lemma CS4_L2:
+"(\<exists> (*CS4_VARIABLESANDTYPES*).
+(PRE4)
+\<and> (PO5)
+\<and> (SI1)
+\<and> (SI1'))"
+sorry
+
+lemma CS6_L3:
+"(\<exists> (*CS5_VARIABLESANDTYPES*).
+(PRE6)
+\<and> (PO7)
+\<and> (SI1)
+\<and> (SI1'))"
+sorry
+
+lemma CS6_L4:
+"(\<exists> (*CS6_VARIABLESANDTYPES*).
+(PRE6)
+\<and> (PO7)
+\<and> (SI1)
+\<and> (SI1'))"
+sorry
+
+lemma CS1_L5:
+"(\<exists> (*CS1_VARIABLESANDTYPES*).
+(PRE1)
+\<and> (PO2)
+\<and> (SI1)
+\<and> (SI1'))"
+sorry
+
+lemma CS3_L6:
+"(\<exists> (*CS3_VARIABLESANDTYPES*).
+(PRE3)
+\<and> (PO4)
+\<and> (SI1)
+\<and> (SI1'))"
+sorry
 
 end
 end
